Proofs for montgomery_reduce_element and montgomery_multiply_fe_by_fer

libcrux-ml-dsa/src/simd/portable/arithmetic.rs
@@ -85,24 +85,109 @@ pub(crate) fn get_n_least_significant_bits(n: u8, value: u64) -> u64 {
 }
 
 #[inline(always)]
+#[hax_lib::fstar::options("--z3rlimit 500 --split_queries always")]
+#[hax_lib::requires(fstar!(r#"Spec.Utils.is_i64b (8380416 * pow2 32) value "#))]
+#[hax_lib::ensures(|result| fstar!(r#"Spec.Utils.is_i32b (8380416 + 4190209) result /\
+                (Spec.Utils.is_i64b (8380416 * pow2 31) value ==> Spec.Utils.is_i32b 8380416 result) /\
+                v result % 8380417 == (v value * 8265825) % 8380417"#))]
 pub(crate) fn montgomery_reduce_element(value: i64) -> FieldElementTimesMontgomeryR {
     let t = get_n_least_significant_bits(MONTGOMERY_SHIFT, value as u64)
         * INVERSE_OF_MODULUS_MOD_MONTGOMERY_R;
+    hax_lib::fstar!(
+        r#"assert (v $t == (v $value % pow2 32) * 58728449)"#
+    );
     let k = get_n_least_significant_bits(MONTGOMERY_SHIFT, t) as i32;
+    hax_lib::fstar!(
+        r#"assert (v $k == v $t @% pow2 32);
+        assert(v (cast ($k <: i32) <: i64) == v $k);
+        assert(v (cast ($k <: i32) <: i64) < pow2 31);
+        assert(v (cast ($k <: i32) <: i64) >= -pow2 31);
+        assert(v (cast ($FIELD_MODULUS <: i32) <: i64) == 8380417)"#
+    );
 
     let k_times_modulus = (k as i64) * (FIELD_MODULUS as i64);
+    hax_lib::fstar!(
+        r#"Spec.Utils.lemma_mul_i32b (pow2 31) (8380417) $k $FIELD_MODULUS;
+        assert (Spec.Utils.is_i64b (pow2 31 * 8380417) $k_times_modulus)"#
+    );
 
     let c = (k_times_modulus >> MONTGOMERY_SHIFT) as i32;
+    hax_lib::fstar!(
+        r#"assert (v $k_times_modulus < pow2 63);
+        assert (v $k_times_modulus / pow2 32 < pow2 31);
+        assert (v $c == (v $k_times_modulus / pow2 32) @% pow2 32);
+        assert(v $c == v $k_times_modulus / pow2 32); 
+        assert(Spec.Utils.is_i32b 4190209 $c)"#
+    );
     let value_high = (value >> MONTGOMERY_SHIFT) as i32;
+    hax_lib::fstar!(
+        r#"assert (v $value < pow2 63);
+        assert (v $value / pow2 32 < pow2 31);
+        assert (v $value_high == (v $value / pow2 32) @% pow2 32);
+        Spec.Utils.lemma_div_at_percent (v $value) (pow2 32);
+        assert (v $value_high == (v $value / pow2 32));
+        assert (Spec.Utils.is_i64b (8380416 * 8380416) $value ==> Spec.Utils.is_i32b 8265825 $value_high);
+        assert(Spec.Utils.is_i32b 8380416 $value_high)"#
+    );
 
-    value_high - c
+    let res = value_high - c;
+    hax_lib::fstar!(
+        r#"assert(Spec.Utils.is_i32b (8380416 + 4190209) $res);
+        assert(Spec.Utils.is_i64b (8380416 * pow2 31) $value ==> Spec.Utils.is_i32b 58728448 $res)"#
+    );
+    hax_lib::fstar!(
+        r#"calc ( == ) {
+            v $k_times_modulus % pow2 32;
+            ( == ) { assert (v $k_times_modulus == v $k * 8380417) }
+            (v $k * 8380417) % pow2 32;
+            ( == ) { assert (v $k = ((v $value % pow2 32) * 58728449) @% pow2 32) }
+            ((((v $value % pow2 32) * 58728449) @% pow2 32) * 8380417) % pow2 32;
+            ( == ) {  Math.Lemmas.lemma_mod_sub ((((v $value % pow2 32) * 58728449) % pow2 32) * 8380417) (pow2 32) 8380417 }
+            ((((v $value % pow2 32) * 58728449) % pow2 32) * 8380417) % pow2 32;
+            ( == ) {  Math.Lemmas.lemma_mod_mul_distr_l ((v $value % pow2 32) * 58728449) 8380417 (pow2 32) }
+            ((((v $value % pow2 32) * 58728449) * 8380417) % pow2 32);
+            ( == ) {  Math.Lemmas.lemma_mod_mul_distr_r (v $value % pow2 32) (58728449 * 8380417) (pow2 32) }
+            ((v $value % pow2 32) % pow2 32);
+            ( == ) { Math.Lemmas.lemma_mod_sub (v $value) (pow2 32) 1 }
+            (v $value) % pow2 32;
+        };
+        Math.Lemmas.modulo_add (pow2 32) (- (v $k_times_modulus)) (v $value) (v $k_times_modulus);
+        assert ((v $value - v $k_times_modulus) % pow2 32 == 0)"#
+    );
+    hax_lib::fstar!(
+        r#"calc ( == ) {
+            v $res % 8380417;
+            ( == ) { assert (v $res == v $value_high - v $c) }
+            (v $value / pow2 32 - v $k_times_modulus / pow2 32) % 8380417;
+            ( == ) { Math.Lemmas.lemma_div_exact (v $value - v $k_times_modulus) (pow2 32) }
+            ((v $value - v $k_times_modulus) / pow2 32) % 8380417;
+            ( == ) { assert ((pow2 32 * 8265825) % 8380417 == 1) }
+            (((v $value - v $k_times_modulus) / pow2 32) * ((pow2 32 * 8265825) % 8380417)) % 8380417;
+            ( == ) { Math.Lemmas.lemma_mod_mul_distr_r ((v $value - v $k_times_modulus) / pow2 32)
+            (pow2 32 * 8265825)
+            8380417 }
+            (((v $value - v $k_times_modulus) / pow2 32) * pow2 32 * 8265825) % 8380417;
+            ( == ) { Math.Lemmas.lemma_div_exact (v $value - v $k_times_modulus) (pow2 32) }
+            ((v $value - v $k_times_modulus) * 8265825) % 8380417;
+            ( == ) { assert (v $k_times_modulus == (v $k @% pow2 32) * 8380417) }
+            ((v $value * 8265825) - ((v $k @% pow2 32) * 8380417 * 8265825)) % 8380417;
+            ( == ) { Math.Lemmas.lemma_mod_sub (v $value * 8265825) 8380417 ((v $k @% pow2 32) * 8265825) }
+            (v $value * 8265825) % 8380417;
+        }"#
+    );
+    res
 }
 
 #[inline(always)]
+#[hax_lib::fstar::options("--z3rlimit 300")]
+#[hax_lib::requires(fstar!(r#"Spec.Utils.is_i32b 4190208 fer"#))]
+#[hax_lib::ensures(|result| fstar!(r#"Spec.Utils.is_i32b 8380416 result /\
+                v result % 8380417 == (v fe * v fer * 8265825) % 8380417"#))]
 pub(crate) fn montgomery_multiply_fe_by_fer(
     fe: FieldElement,
     fer: FieldElementTimesMontgomeryR,
 ) -> FieldElement {
+    hax_lib::fstar!(r#"Spec.Utils.lemma_mul_i32b (pow2 31) (4190208) fe fer"#);
     montgomery_reduce_element((fe as i64) * (fer as i64))
 }
 
