libcrux-ml-dsa/proofs/fstar/spec/Spec.Utils.fst
@@ -1,0 +1,58 @@
+module Spec.Utils
+#set-options "--fuel 0 --ifuel 1 --z3rlimit 100"
+open FStar.Mul
+open Core
+
+#push-options "--z3rlimit 100 --split_queries always"
+let lemma_range_at_percent (v:int) (p:int{p>0/\ p%2=0 /\ v < p/2 /\ v >= -p / 2}):
+  Lemma (v @% p == v) =
+    let m = v % p in
+    if v < 0 then (
+      Math.Lemmas.lemma_mod_plus v 1 p;
+      assert ((v + p) % p == v % p);
+      assert (v + p >= 0);
+      assert (v + p < p);
+      Math.Lemmas.modulo_lemma (v+p) p;
+      assert (m == v + p);
+      assert (m >= p/2);
+      assert (v @% p == m - p);
+      assert (v @% p == v))
+    else (
+      assert (v >= 0 /\ v < p);
+      Math.Lemmas.modulo_lemma v p;
+      assert (v % p == v);
+      assert (m < p/2);
+      assert (v @% p == v)
+    )
+#pop-options
+
+let lemma_div_at_percent (v:int) (p:int{p>0/\ p%2=0 /\ (v/p) < p/2 /\ (v/p) >= -p / 2}):
+  Lemma ((v / p) @% p == v / p) = 
+    lemma_range_at_percent (v/p) p
+
+/// Bounded integers
+
+let is_intb (l:nat) (x:int) = (x <= l) && (x >= -l)
+
+let is_i32b (l:nat) (x:i32) = is_intb l (v x)
+let is_i64b (l:nat) (x:i64) = is_intb l (v x)
+
+#push-options "--z3rlimit 200"
+val lemma_mul_i32b (b1 b2: nat) (n1 n2: i32) 
+    : Lemma (requires (is_i32b b1 n1 /\ is_i32b b2 n2 /\ b1 * b2 < pow2 63))
+      (ensures (range (v n1 * v n2) i64_inttype /\ 
+                is_i64b (b1 * b2) ((cast n1 <: i64) *! (cast n2 <: i64)) /\
+                v ((cast n1 <: i64) *! (cast n2 <: i64)) == v n1 * v n2))
+      
+let lemma_mul_i32b (b1 b2: nat) (n1 n2: i32) =
+  if v n1 = 0 || v n2 = 0
+  then ()
+  else 
+    let open FStar.Math.Lemmas in
+    lemma_abs_bound (v n1) b1;
+    lemma_abs_bound (v n2) b2;
+    lemma_abs_mul (v n1) (v n2);
+    lemma_mult_le_left (abs (v n1)) (abs (v n2)) b2;
+    lemma_mult_le_right b2 (abs (v n1)) b1;
+    lemma_abs_bound (v n1 * v n2) (b1 * b2)
+#pop-options
